\def\newstep#1{\smallskip \noindent {\bf #1}}
\def\newhead#1{\vskip 0.1in \noindent {\bf #1}}

\topglue 0.5in
\centerline{Notes on Knuth Fascicle 5a: Mathematical Preliminaries Redux}
\vskip 0.3in

\noindent{\bf Inequalities}

\noindent [p 5] Formula (23): derivation of the second moment principle.  The
final step again takes advantage of ${\rm E}\left(X | X > 0\right) = {\rm E} \left(X | X > 0\right)
{\rm Pr}\left(X > 0\right) + {\rm E} \left(X | X = 0\right) {\rm Pr}\left(X = 0\right) = {\rm E} \left(X | X > 0\right)
{\rm Pr}\left(X > 0\right)$, and therefore $\left( {\rm E} \left(X | X > 0\right) \right)^2 = 
\left({\rm E} \left(X \right) / {\rm Pr}\left(X > 0\right) \right)^2$.

\bye